theories/automation.v
@@ -1,0 +1,192 @@
+From iris.proofmode Require Import coq_tactics reduction.
+From isla Require Export lifting.
+From refinedc.lithium Require Export lithium tactics.
+Set Default Proof Using "Type".
+
+(** * Registering extensions *)
+(** More automation for modular arithmetics. *)
+Ltac Zify.zify_post_hook ::= Z.to_euclidean_division_equations.
+
+Section instances.
+  Context `{!islaG Σ} `{!threadG}.
+
+  Global Instance instr_intro_pers i a : IntroPersistent (instr a i) (instr a i).
+  Proof. constructor. iIntros "#$". Qed.
+
+  Global Instance reg_extern_intro_pers r : IntroPersistent (r ↦ᵣ !) (r ↦ᵣ !).
+  Proof. constructor. iIntros "#$". Qed.
+
+  Definition FindReg (r : register_name) := {|
+    fic_A := option valu; fic_Prop ov := if ov is Some v then r ↦ᵣ v else r ↦ᵣ ! ;
+  |}%I.
+  Typeclasses Opaque FindReg.
+
+  Lemma find_in_context_reg_local r G:
+     (∃ v, r ↦ᵣ v ∗ G (Some v)) -∗
+    find_in_context (FindReg r) G.
+  Proof. iDestruct 1 as (?) "[Hr HG]". iExists _. by iFrame. Qed.
+  Global Instance find_in_context_reg_local_inst r :
+    FindInContext (FindReg r) 0%nat FICSyntactic :=
+    λ G, i2p (find_in_context_reg_local r G).
+
+  Lemma find_in_context_reg_extern r G:
+     (r ↦ᵣ ! ∗ G None) -∗
+    find_in_context (FindReg r) G.
+  Proof. iDestruct 1 as "[Hr HG]". iExists _. by iFrame. Qed.
+  Global Instance find_in_context_reg_extern_inst r :
+    FindInContext (FindReg r) 1%nat FICSyntactic :=
+    λ G, i2p (find_in_context_reg_extern r G).
+
+  Global Instance reg_related r v : RelatedTo (r ↦ᵣ v) := {|
+    rt_fic := FindDirect (λ v, r ↦ᵣ v)%I;
+  |}.
+
+  Global Instance instr_related a i : RelatedTo (instr a i) := {|
+    rt_fic := FindDirect (λ i, instr a i)%I;
+  |}.
+
+  Global Instance spec_trace_related κs : RelatedTo (spec_trace κs) := {|
+    rt_fic := FindDirect (λ κs, spec_trace κs)%I;
+  |}.
+
+  Lemma subsume_reg r v1 v2 G:
+    ⌜v1 = v2⌝ ∗ G -∗
+    subsume (r ↦ᵣ v1) (r ↦ᵣ v2) G.
+  Proof. iDestruct 1 as (->) "$". iIntros "$". Qed.
+  Global Instance subsume_reg_inst r v1 v2 :
+    Subsume (r ↦ᵣ v1) (r ↦ᵣ v2) :=
+    λ G, i2p (subsume_reg r v1 v2 G).
+
+  Lemma subsume_instr a i1 i2 G:
+    ⌜i1 = i2⌝ ∗ G -∗
+    subsume (instr a i1) (instr a i2) G.
+  Proof. iDestruct 1 as (->) "$". iIntros "$". Qed.
+  Global Instance subsume_instr_inst a i1 i2 :
+    Subsume (instr a i1) (instr a i2) :=
+    λ G, i2p (subsume_instr a i1 i2 G).
+
+  Lemma subsume_spec_trace κs1 κs2 G:
+    ⌜κs1 = κs2⌝ ∗ G -∗
+    subsume (spec_trace κs1) (spec_trace κs2) G.
+  Proof. iDestruct 1 as (->) "$". iIntros "$". Qed.
+  Global Instance subsume_spec_trace_inst κs1 κs2 :
+    Subsume (spec_trace κs1) (spec_trace κs2) :=
+    λ G, i2p (subsume_spec_trace κs1 κs2 G).
+
+
+  Lemma li_wp_next_instr:
+    (∃ nPC bPC_changed, "_PC" ↦ᵣ Val_Bits nPC ∗ "__PC_changed" ↦ᵣ Val_Bool bPC_changed ∗
+     ∃ a newPC newPC_changed, ⌜next_pc nPC bPC_changed = Some (a, newPC, newPC_changed)⌝ ∗
+     ∃ ins, instr a ins ∗
+     match ins with
+     | Some ts =>
+       ⌜ts ≠ []⌝ ∗ [∧ list] t∈ts, "_PC" ↦ᵣ newPC -∗ "__PC_changed" ↦ᵣ newPC_changed -∗ WPasm t
+     | None =>
+       ∃ vR0 vR1 vR30 κs, "R0" ↦ᵣ vR0 ∗ "R1" ↦ᵣ vR1 ∗ "R30" ↦ᵣ vR30 ∗ spec_trace κs ∗
+          ⌜hd_error κs = Some (SInstrTrap a
+            {| _PC := newPC; __PC_changed := newPC_changed; R0 := vR0; R1 := vR1; R30 := vR30 |})⌝
+                              ∗ True
+     end
+    ) -∗
+    WPasm [].
+  Proof.
+    iDestruct 1 as (??) "(?&?&Hwp)".
+    iDestruct "Hwp" as (???? ins) "[Hi Hwp]".
+    case_match.
+    - iDestruct "Hwp" as (?) "Hl".
+      iApply (wp_next_instr with "[$] [$] [$]") => //.
+      iIntros (i Hi) "? ?".
+      iDestruct (big_andL_elem_of with "Hl") as "Hwp"; [done|].
+      iApply ("Hwp" with "[$] [$]").
+    - iDestruct "Hwp" as (????) "(?&?&?&?&%&?)".
+      iApply (wp_next_instr_extern with "[$] [$] [$] [$] [$] [$] [$]") => //.
+  Qed.
+
+  Lemma li_wp_read_reg r v ann es:
+    (∃ v', r ↦ᵣ v' ∗ (⌜v = v'⌝ -∗ r ↦ᵣ v' -∗ WPasm es)) -∗
+    WPasm (ReadReg r [] v ann :: es).
+  Proof. iDestruct 1 as (?) "[Hr Hwp]". by iApply (wp_read_reg with "Hr"). Qed.
+
+  Lemma li_wp_write_reg r f v ann es:
+    find_in_context (FindReg r) (λ ov,
+      if ov is Some v' then
+        ⌜f = []⌝ ∗ (r ↦ᵣ v -∗ WPasm es)
+      else
+        ∃ κs, spec_trace κs ∗
+              ⌜head κs = Some (SWriteReg r f v)⌝ ∗
+              (spec_trace (tail κs) -∗ WPasm es)
+     ) -∗
+    WPasm (WriteReg r f v ann :: es).
+  Proof.
+    iDestruct 1 as (?) "[Hr Hwp]". case_match; simplify_eq/=.
+    - iDestruct "Hwp" as (->) "Hwp".
+      by iApply (wp_write_reg with "Hr").
+    - iDestruct "Hwp" as ([|??]) "(?&%&Hwp)" => //. simplify_eq/=.
+      by iApply (wp_write_reg_extern with "Hr [$]").
+  Qed.
+
+  Lemma li_wp_branch_address v ann es:
+    WPasm es -∗
+    WPasm (BranchAddress v ann :: es).
+  Proof. apply: wp_branch_address. Qed.
+
+  Lemma li_wp_declare_const_bv v es ann b:
+    (∀ n, WPasm ((subst_event v (Val_Bits [BV{b} n])) <$> es)) -∗
+    WPasm (Smt (DeclareConst v (Ty_BitVec b)) ann :: es).
+  Proof. apply: wp_declare_const_bv. Qed.
+
+  Lemma li_wp_define_const n es ann e:
+    WPexp e {{ v, WPasm ((subst_event n v) <$> es) }} -∗
+    WPasm (Smt (DefineConst n e) ann :: es).
+  Proof. apply: wp_define_const. Qed.
+
+  Lemma li_wpe_val v Φ ann:
+    Φ v -∗
+    WPexp (Val v ann) {{ Φ }}.
+  Proof. apply: wpe_val. Qed.
+
+  Lemma li_wpe_manyop op es Φ ann:
+    foldr (λ e Ψ, λ vs, WPexp e {{ v, Ψ (vs ++ [v]) }}) (λ vs, ∃ v, ⌜eval_manyop op vs = Some v⌝ ∗ Φ v) es [] -∗
+    WPexp (Manyop op es ann) {{ Φ }}.
+  Proof. apply: wpe_manyop. Qed.
+
+End instances.
+
+Ltac liAAsm :=
+  lazymatch goal with
+  | |- envs_entails ?Δ (WPasm ?es) =>
+    lazymatch es with
+    | [] => notypeclasses refine (tac_fast_apply (li_wp_next_instr) _)
+    | ?e :: _ =>
+      lazymatch e with
+      | ReadReg _ _ _ _ => notypeclasses refine (tac_fast_apply (li_wp_read_reg _ _ _ _) _)
+      | WriteReg _ _ _ _ => notypeclasses refine (tac_fast_apply (li_wp_write_reg _ _ _ _ _) _)
+      | BranchAddress _ _ => notypeclasses refine (tac_fast_apply (li_wp_branch_address _ _ _) _)
+      | Smt (DeclareConst _ (Ty_BitVec _)) _ => notypeclasses refine (tac_fast_apply (li_wp_declare_const_bv _ _ _ _) _)
+      | Smt (DefineConst _ _) _ => notypeclasses refine (tac_fast_apply (li_wp_define_const _ _ _ _) _)
+      end
+    | ?def => first [
+                 iEval (unfold def)
+               | fail "liAAsm: unknown asm" es
+               ]
+    end
+  end.
+
+Ltac liAExp :=
+  lazymatch goal with
+  | |- envs_entails ?Δ (wp_exp ?e _) =>
+    lazymatch e with
+    | Val _ _ => notypeclasses refine (tac_fast_apply (li_wpe_val _ _ _) _)
+    | Manyop _ _ _ => notypeclasses refine (tac_fast_apply (li_wpe_manyop _ _ _ _) _)
+    | _ => fail "liAExp: unknown exp" e
+    end
+  end.
+
+
+Ltac liAStep :=
+ liEnforceInvariantAndUnfoldInstantiatedEvars;
+ first [
+    liAAsm
+  | liAExp
+  | liStep
+]; liSimpl.
