theories/base.v
@@ -2,6 +2,7 @@ From Coq Require Export ssreflect.
 From stdpp Require Export prelude strings gmap.
 From RecordUpdate Require Export RecordSet.
 From refframe Require Export module.
+From refinedc.lang Require Export base.
 Export RecordSetNotations.
 
 Open Scope Z_scope.
